LL1/ParseTableGen.v
@@ -1,44 +1,39 @@
 Require Import List.
+Require Import Nat Ndec NArith.
 
 Require Import Lib.Grammar.
 Require Import Lib.Lemmas.
 Require Import Lib.Tactics.
 
+Require Import LL1.Lemmas.
 Require Import LL1.ParseTable.
 
 Import ListNotations.
 
 Definition prod_la_pair := (production * lookahead)%type.
 
-Definition singletonLaMap la gamma :=
-  LaMap.add la gamma (LaMap.empty (list symbol)).
+Definition empty_pt := ParseTable.empty (list symbol).
 
-Definition empty_pt := NtMap.empty (LaMap.t (list symbol)).
-
-Definition pairs_wf ps g :=
-  forall x gamma la,
-    In ((x, gamma), la) ps <-> lookahead_for la x gamma g.
-
-Definition addEntry (p : prod_la_pair) o :=
+Definition addEntry (p : prod_la_pair) (o : option parse_table) :=
   match o with
   | None => None
   | Some tbl =>
     match p with
     | ((x, gamma), la) =>
-      match NtMap.find x tbl with
-      | None => Some (NtMap.add x (singletonLaMap la gamma) tbl)
-      | Some m =>
-        match LaMap.find la m with
-        | None => Some (NtMap.add x (LaMap.add la gamma m) tbl)
-        | Some gamma' =>
-          if list_eq_dec symbol_eq_dec gamma gamma' then Some tbl else None
-        end
+      match pt_lookup x la tbl with
+      | None => Some (pt_add x la gamma tbl)
+      | Some gamma' =>
+        if list_eq_dec symbol_eq_dec gamma gamma' then Some tbl else None (* make separate function *)
       end
     end
   end.
 
 Definition mkParseTable (ps : list prod_la_pair) :=
   fold_right addEntry (Some empty_pt) ps.
+
+Definition pairs_wf ps g :=
+  forall x gamma la,
+    In ((x, gamma), la) ps <-> lookahead_for la x gamma g.
 
 Definition tbl_correct_wrt_pairs tbl ps :=
   forall x gamma la,
@@ -89,66 +84,118 @@ Proof.
   - unfold addEntry in Hadd; inv Hadd.
 Qed.
 
+Lemma duplicate_preserves_invariant :
+  forall tbl ps x la gamma,
+    tbl_correct_wrt_pairs tbl ps
+    -> pt_lookup x la tbl = Some gamma
+    -> tbl_correct_wrt_pairs tbl (((x, gamma), la) :: ps).
+Proof.
+  intros tbl ps x la gamma Htc Hlk.
+  unfold tbl_correct_wrt_pairs.
+  intros x' gamma' la'.
+  split.
+  - intros Hlk'.
+    unfold tbl_correct_wrt_pairs in Htc.
+    apply Htc in Hlk'.
+    right; auto.
+  - intros Hin.
+    inv Hin.
+    + inv H; auto.
+    + apply Htc; auto.
+Qed.
+
+Lemma lookup_add_or :
+  forall x x' la la' gamma gamma' tbl,
+    pt_lookup x' la' (pt_add x la gamma tbl) = Some gamma'
+    -> (x = x' /\ la = la' /\ gamma = gamma')
+       \/ pt_lookup x' la' tbl = Some gamma'.
+Proof.
+  intros x x' la la' gamma gamma' tbl Hlk.
+  unfold pt_lookup in Hlk; unfold pt_add in Hlk.
+  rewrite ParseTableFacts.add_o in Hlk.
+  destruct (ParseTableFacts.eq_dec (x, la) (x', la')).
+  - inv e.
+    inv Hlk.
+    left; auto.
+  - right; auto.
+Qed.
+
+Lemma new_entry_preserves_invariant :
+  forall tbl ps x la gamma,
+    tbl_correct_wrt_pairs tbl ps
+    -> pt_lookup x la tbl = None
+    -> tbl_correct_wrt_pairs (pt_add x la gamma tbl) (((x, gamma), la) :: ps).
+Proof.
+  intros tbl ps x la gamma Htc Hlk.
+  unfold tbl_correct_wrt_pairs.
+  intros x' gamma' la'.
+  split.
+  - intros Hlk'.
+    apply lookup_add_or in Hlk'.
+    inv Hlk'.
+    + destruct H as [Hx [Hla Hgamma]]; subst.
+      left; auto.
+    + apply Htc in H.
+      right; auto.
+  - intros Hin.
+    inv Hin.
+    + inv H.
+      unfold pt_lookup.
+      unfold pt_add.
+      apply ParseTableFacts.add_eq_o; auto.
+    + apply Htc in H.
+      destruct (ParseTableFacts.eq_dec (x, la) (x', la')). 
+      * inv e; congruence.
+      * unfold pt_lookup.
+        unfold pt_add.
+        rewrite ParseTableFacts.add_neq_o; auto.
+Qed.
+
 Lemma addEntry_preserves_invariant :
   forall p ps tbl' tbl,
     tbl_correct_wrt_pairs tbl' ps
     -> addEntry p (Some tbl') = Some tbl
     -> tbl_correct_wrt_pairs tbl (p :: ps).
 Proof.
-  intros p ps tbl' tbl Htc Hadd.
-  destruct p as ((x, gamma), la).
+  intros ((x, gamma), la) ps tbl' tbl Htc Hadd.
+  unfold addEntry in Hadd.
+  destruct (pt_lookup x la tbl') as [gamma' |] eqn:Hlk.
+  - destruct (list_eq_dec symbol_eq_dec gamma gamma').
+    + inv e.
+      inv Hadd.
+      apply duplicate_preserves_invariant; auto.
+    + inv Hadd.
+  - inv Hadd.
+    apply new_entry_preserves_invariant; auto.
+Qed.
+
+Lemma empty_table_correct_wrt_empty_pairs :
+  tbl_correct_wrt_pairs empty_pt [].
+Proof.
   unfold tbl_correct_wrt_pairs.
-  intros x' gamma' la'.
+  intros x gamma la.
   split.
   - intros Hlk.
-    simpl in Hadd.
-    unfold addEntry in Hadd.
-    destruct (NtMap.find x tbl') as [m |] eqn:Hnf.
-    + destruct (LaMap.find la m) as [gamma'' |] eqn:Hlf.
-      * destruct (list_eq_dec symbol_eq_dec gamma gamma'').
+    unfold pt_lookup in Hlk.
+    rewrite ParseTableFacts.empty_o in Hlk; inv Hlk.
+  - intros Hin; inv Hin.
+Qed.
 
-Admitted.
-
-Lemma mkParseTable_satisfies_invariant :
+Lemma mkParseTable_sound_wrt_invariant :
   forall ps tbl,
-         (* pairs_wf ps g *) (* this has to be global, not inductive *)
     mkParseTable ps = Some tbl
     -> tbl_correct_wrt_pairs tbl ps.
 Proof.
   intros ps.
   induction ps as [| p ps]; intros tbl Hmk; simpl in *.
   - inv Hmk.
-    admit.
+    apply empty_table_correct_wrt_empty_pairs.
   - pose proof Hmk as Hmk'.
     apply addEntry_preserves_Some in Hmk.
     destruct Hmk as [tbl' Hmk].
     rewrite Hmk in Hmk'.
     eapply addEntry_preserves_invariant; eauto.
-Admitted.
-
-(*
-  intros ps g Hwf.
-  induction ps as [| p ps]; intros tbl Hmk; simpl in *.
-  - inv Hmk.
-    unfold tbl_correct_wrt_pairs.
-    split.
-    + unfold tbl_sound_wrt_pairs.
-      intros x gamma la Hlk.
-      unfold pt_lookup in Hlk.
-      destruct (NtMap.find x empty_pt) eqn:Hnf.
-      * rewrite NtMapFacts.empty_o in Hnf; inv Hnf.
-      * inv Hlk.
-    + unfold tbl_complete_wrt_pairs.
-      intros x gamma la laSet Hin; inv Hin.
-  - pose proof Hmk as Hmk'.
-    apply addEntries_preserves_Some in Hmk.
-    destruct Hmk as [tbl' Hmk].
-    rewrite Hmk in Hmk'.
-    inv Hwf.
-    destruct p as ((x, gamma), laSet).
-    eapply addEntries_preserves_invariant; eauto.
 Qed.
- *)
 
 Lemma mkParseTable_sound :
   forall ps g tbl,
@@ -158,375 +205,6 @@ Lemma mkParseTable_sound :
 Proof.
   intros ps g tbl Hwf Hmk.
   eapply invariant_iff_parse_table_for; eauto.
-  eapply mkParseTable_satisfies_invariant; eauto.
+  eapply mkParseTable_sound_wrt_invariant; eauto.
 Qed.      
-      
-(*
-Definition tbl_sound_wrt_pairs tbl ps :=
-  forall x gamma la,
-    pt_lookup x la tbl = Some gamma
-    -> exists laSet,
-      In ((x, gamma), laSet) ps /\ LaSet.In la laSet.
 
-Definition tbl_complete_wrt_pairs tbl ps :=
-  forall x gamma la laSet,
-    In ((x, gamma), laSet) ps
-    -> LaSet.In la laSet
-    -> pt_lookup x la tbl = Some gamma.
-
-Definition tbl_correct_wrt_pairs tbl ps :=
-  tbl_sound_wrt_pairs tbl ps /\ tbl_complete_wrt_pairs tbl ps.
-
-Lemma invariant_iff_parse_table_for :
-  forall g ps tbl,
-    g.(productions) = map fst ps
-    -> prod_la_pairs_wf ps g
-    -> tbl_correct_wrt_pairs tbl ps
-       <-> parse_table_for tbl g.
-Proof.
-  intros g ps tbl Heq Hwf.
-  split.
-  - intros Hinv.
-    destruct Hinv as [Hts Htc].
-    unfold parse_table_for.
-    split.
-    + unfold pt_sound.
-      intros x la gamma Hlk.
-      unfold tbl_sound_wrt_pairs in Hts.
-      apply Hts in Hlk.
-      destruct Hlk as [laSet [Hpin Hlin]].
-      unfold prod_la_pairs_wf in Hwf.
-      rewrite Forall_forall in Hwf.
-      apply Hwf in Hpin.
-      unfold prod_la_pair_wf in Hpin.
-      unfold lookahead_set_for in Hpin.
-      destruct Hpin; auto.
-    + unfold pt_complete.
-      intros la x gamma Hlk.
-      pose proof Hlk as Hlk'.
-      unfold lookahead_for in Hlk.
-      destruct Hlk as [Hin Hlk].
-      pose proof in_map_iff.
-      specialize H with (y := (x, gamma)) (f := fst) (l := ps).
-      rewrite <- Heq in H.
-      apply H in Hin.
-      destruct Hin as [pr [Hfst Hin]].
-      destruct pr as (prod, laSet).
-      destruct prod as (y, gamma').
-      inv Hfst.
-      unfold tbl_complete_wrt_pairs in Htc.
-      eapply Htc; eauto.
-      unfold prod_la_pairs_wf in Hwf.
-      rewrite Forall_forall in Hwf.
-      apply Hwf in Hin.
-      inv Hin.
-      apply H1; auto.
-  - intros Hpt.
-    unfold tbl_correct_wrt_pairs.
-    destruct Hpt as [Hsou Hcom].
-    split.
-    + unfold tbl_sound_wrt_pairs.
-      intros x gamma la Hlk.
-      pose proof Hlk as Hlk'.
-      unfold pt_sound in Hsou.
-      apply Hsou in Hlk.
-      unfold prod_la_pairs_wf in Hwf.
-      rewrite Forall_forall in Hwf.
-      destruct Hlk as [Hin Hlk].
-      pose proof in_map_iff.
-      specialize H with (y := (x, gamma)) (f := fst) (l := ps).
-      rewrite <- Heq in H.
-      apply H in Hin.
-      destruct Hin as [pr [Hfst Hin]].
-      destruct pr as (prod, laSet).
-      destruct prod as (y, gamma').
-      inv Hfst.
-      pose proof Hin as Hin'.
-      apply Hwf in Hin.
-      unfold prod_la_pair_wf in Hin.
-      unfold lookahead_set_for in Hin.
-      destruct Hin as [Hls Hlc].
-      exists laSet; split; auto.
-    + unfold tbl_complete_wrt_pairs.
-      intros x gamma la laSet Hin Hla.
-      unfold pt_complete in Hcom.
-      apply Hcom.
-      unfold prod_la_pairs_wf in Hwf.
-      rewrite Forall_forall in Hwf.
-      apply Hwf in Hin.
-      unfold prod_la_pair_wf in Hin.
-      destruct Hin.
-      apply H; auto.
-Qed.
-
-Definition prod_la_pair := (production * LaSet.t)%type.
-
-Definition prod_la_pair_wf (g : grammar) (p : prod_la_pair) :=
-  match p with
-  | ((x, gamma), laSet) => lookahead_set_for laSet x gamma g
-  end.
-
-Definition prod_la_pairs_wf (ps : list prod_la_pair) (g : grammar) :=
-  Forall (prod_la_pair_wf g) ps.
-
-Definition empty_pt := NtMap.empty (LaMap.t (list symbol)).
-
-Definition singletonLaMap la gamma :=
-  LaMap.add la gamma (LaMap.empty (list symbol)).
-  
-Definition addEntry (x : nonterminal) (la : lookahead) (gamma : list symbol) (o : option parse_table) :=
-  match o with
-  | None => None
-  | Some tbl => 
-    match NtMap.find x tbl with
-    | None => Some (NtMap.add x (singletonLaMap la gamma) tbl)
-    | Some m =>
-      match LaMap.find la m with
-      | None => Some (NtMap.add x (LaMap.add la gamma m) tbl)
-      | Some gamma' =>
-        if list_eq_dec symbol_eq_dec gamma gamma' then Some tbl else None
-      end
-    end
-  end.
-
-Definition addEntries (p : prod_la_pair) (o : option parse_table) :=
-  match p with
-  | ((x, gamma), laSet) =>
-    fold_right (fun la o => addEntry x la gamma o) o (LaSet.elements laSet)
-  end.
-
-Definition mkParseTable (productions_with_la_sets : list prod_la_pair) :=
-  fold_right addEntries (Some empty_pt) productions_with_la_sets.
-
-Lemma addEntry_None_eq_None :
-  forall x la gamma,
-    addEntry x la gamma None = None.
-Proof.
-  auto.
-Qed.
-
-Lemma addEntry_preserves_Some :
-  forall x la gamma o tbl,
-    addEntry x la gamma o = Some tbl
-    -> exists tbl',
-      o = Some tbl'.
-Proof.
-  intros x la gamma o tbl Hadd.
-  unfold addEntry in Hadd.
-  destruct o as [tbl' |] eqn:Ho.
-  - exists tbl'; auto.
-  - inv Hadd.
-Qed.
-
-Lemma addEntries_None_eq_None :
-  forall p,
-    addEntries p None = None.
-Proof.
-  intros p.
-  destruct p as ((x, gamma), laSet); simpl.
-  induction (LaSet.elements laSet); simpl; auto.
-  rewrite IHl.
-  apply addEntry_None_eq_None.
-Qed.
-
-Lemma addEntries_preserves_Some :
-  forall p ps tbl,
-    addEntries p (mkParseTable ps) = Some tbl
-    -> exists tbl',
-      mkParseTable ps = Some tbl'.
-Proof.
-  intros.
-  destruct (mkParseTable ps) as [tbl' |].
-  + exists tbl'; auto.
-  + rewrite addEntries_None_eq_None in H; inv H.
-Qed.
-
-Lemma empty_laSet_preserves_invariant :
-  forall tbl ps x gamma s,
-    tbl_correct_wrt_pairs tbl ps
-    -> LaSet.Empty s
-    -> tbl_correct_wrt_pairs tbl ((x, gamma, s) :: ps).
-Proof.
-  intros tbl ps x gamma s Htc Hem.
-  unfold tbl_correct_wrt_pairs.
-  split.
-  - unfold tbl_sound_wrt_pairs.
-    intros x' gamma' la Hlk.
-    destruct Htc as [Hsou Hcom].
-    apply Hsou in Hlk.
-    destruct Hlk as [s' [Hin Hlin]].
-    exists s'; split; auto.
-    right; auto.
-  - unfold tbl_complete_wrt_pairs.
-    intros x' gamma' la s' Hin Hlin.
-    inv Hin.
-    + inv H.
-      exfalso.
-      eapply Hem; eauto.
-    + destruct Htc as [_ Hcom].
-      eapply Hcom in H; eauto.
-Qed.
-
-Lemma addEntries_thang :
-  forall la laSet x gamma o tbl,
-    addEntries ((x, gamma), laSet) o = Some tbl
-    -> LaSet.In la laSet
-    -> pt_lookup x la tbl = Some gamma.
-Proof.
-  intros la laSet.
-  remember (LaSet.elements laSet) as elts.
-  generalize dependent laSet.
-  induction elts as [| e es].
-  - intros laSet Helts x gamma o tbl Hadd Hin.
-    admit.
-  - intros laSet Helts x gamma o tbl Hadd Hin.
-    pose proof Hadd as Hadd'.
-    unfold addEntries in Hadd.
-    rewrite <- Helts in Hadd; simpl in Hadd.
-    apply addEntry_preserves_Some in Hadd.
-    destruct Hadd as [tbl' Hfr].
-    unfold addEntries in IHes.
-    
-s    
-
-Lemma or_thing :
-  forall tbl' tbl ps x gamma laSet,
-    tbl_correct_wrt_pairs tbl' ps
-    -> addEntries ((x, gamma), laSet) (Some tbl') = Some tbl
-    -> (forall la,
-           LaSet.In la laSet -> pt_lookup x la tbl = Some gamma)
-    -> tbl_correct_wrt_pairs tbl ((x, gamma, laSet) :: ps).
-Proof.
-  intros.
-  unfold tbl_correct_wrt_pairs.
-  split.
-  - unfold tbl_sound_wrt_pairs.
-    intros x' gamma' la Hlk.
-    destruct H as [Hsou Hcom].
-    apply Hsou in Hlk.
-    destruct Hlk as [laSet' [Hin Hlin]].
-    exists laSet'; split; auto.
-    right; auto.
-  - unfold tbl_complete_wrt_pairs.
-    intros x' gamma' la laSet' Hin Hlin.
-    inv Hin.
-    + inv H1; auto.
-    + destruct H as [_ Hcom].
-      eapply Hcom in H1; eauto.
-Qed.
-            
-Lemma addEntries_preserves_invariant :
-  forall laSet x gamma
-         (tbl' tbl : parse_table)
-         (ps : list prod_la_pair),
-    tbl_correct_wrt_pairs tbl' ps
-    -> addEntries ((x, gamma), laSet) (Some tbl') = Some tbl
-    -> tbl_correct_wrt_pairs tbl (((x, gamma), laSet) :: ps).
-Proof.
-  intros.
-  intros laSet.
-  remember (LaSet.elements laSet) as elts.
-  generalize dependent laSet.
-  induction elts as [| e es].
-  - intros laSet Helts x gamma tbl' tbl ps Htc Hadd.
-    eapply empty_laSet_preserves_invariant.
-    + simpl in Hadd.
-      rewrite <- Helts in Hadd; simpl in Hadd.
-      inv Hadd; auto.
-    + apply LaSetEqProps.MP.elements_Empty; auto.
-  - intros laSet Helts x gamma tbl' tbl ps Htc Hadd.
-    
-Admitted.
- *)
-
-Lemma mkParseTable_satisfies_invariant :
-  forall ps g,
-    prod_la_pairs_wf ps g
-    -> forall tbl,
-      mkParseTable ps = Some tbl
-      -> tbl_correct_wrt_pairs tbl ps.
-Proof.
-  intros ps g Hwf.
-  induction ps as [| p ps]; intros tbl Hmk; simpl in *.
-  - inv Hmk.
-    unfold tbl_correct_wrt_pairs.
-    split.
-    + unfold tbl_sound_wrt_pairs.
-      intros x gamma la Hlk.
-      unfold pt_lookup in Hlk.
-      destruct (NtMap.find x empty_pt) eqn:Hnf.
-      * rewrite NtMapFacts.empty_o in Hnf; inv Hnf.
-      * inv Hlk.
-    + unfold tbl_complete_wrt_pairs.
-      intros x gamma la laSet Hin; inv Hin.
-  - pose proof Hmk as Hmk'.
-    apply addEntries_preserves_Some in Hmk.
-    destruct Hmk as [tbl' Hmk].
-    rewrite Hmk in Hmk'.
-    inv Hwf.
-    destruct p as ((x, gamma), laSet).
-    eapply addEntries_preserves_invariant; eauto.
-Qed.
-
-Lemma mkParseTable_sound :
-  forall ps g tbl,
-    g.(productions) = map fst ps
-    -> prod_la_pairs_wf ps g
-    -> mkParseTable ps = Some tbl
-    -> parse_table_for tbl g.
-Proof.
-  intros ps g tbl Hfst Hwf Hmk.
-  eapply invariant_iff_parse_table_for; eauto.
-  eapply mkParseTable_satisfies_invariant; eauto.
-Qed.
-  
-Lemma mkParseTable_correct : 
-  forall (ps : list prod_la_pair)
-         (tbl : parse_table)
-         (g : grammar),
-    prod_la_pairs_wf g ps
-    -> mkParseTable ps = Some tbl
-       <-> parse_table_for tbl g.
-Proof.
-  intros ps tbl g Hwf.
-  split.
-  - (* prove mkParseTable sound -- if it returns parse table tbl,
- tbl is a parse table for g *)
-    intros Hmk.
-    apply tbl_correct_for_pl_pairs_parse_table_for with
-        (ps := ps).
-    
-
-(*
-Lemma mkParseTable_correct : 
-  forall (productions_and_la_sets : list (production * LaSet.t))
-         (tbl : parse_table),
-    -> mkParseTable productions_and_la_sets = Some tbl
-    -> forall (start : nonterminal)
-              (productions : list production),
-        productions = map fst productions_and_la_sets
-        (* productions_and_la_sets is well-formed *)
-        -> 
-       <-> parse_table_for tbl g.
-Proof.
-  intros; split.
-  - revert g tbl H.
-    induction productions_and_la_sets.
-    + (* empty list of productions and lookahead sets --
-         the grammar's productions must be empty, so mkParseTable should return 
-         an empty table *)
-      intros g tbl Hprods Hmk.
-      simpl in *.
-      inv Hmk.
-      unfold parse_table_for; split.
-      * unfold pt_minimal; intros x la gamma laMap Hnf Hlf.
-        exfalso; eapply NtMapFacts.empty_in_iff.
-        apply ntmap_find_in in Hnf; eauto.
-      * unfold pt_complete; intros x la gamma Hlf.
-        exfalso.
-        unfold lookahead_for in Hlf.
-        destruct Hlf as [Hin _].
-        rewrite Hprods in Hin; inv Hin.
-    + intros g tbl Hprods Hmk.
-      destruct a as [[x gamma] laSet].
-*)
